ANF uncurrying

theories/L6_PCPS/uncurry_proto.v
@@ -18,7 +18,8 @@ Unset Strict Unquote Universe Mode.
 
 (** * Auxiliary data used by the rewriter *)
 
-Definition R_misc : Set := unit.
+(* true if in cps mode *)
+Definition R_misc : Set := bool.
 
 (* pair of 
    1 - max number of arguments 
@@ -73,6 +74,7 @@ Definition set_names_lst olds news suff cdata :=
   fold_right (fun '(old, new) cdata => set_name old new suff cdata) cdata (combine olds news).
 
 Inductive uncurry_step : exp -> exp -> Prop :=
+(* Uncurrying for CPS *)
 | uncurry_cps :
   forall (C : frames_t exp_univ_fundefs exp_univ_exp)
     (f f1 : var) (ft ft1 : fun_tag) (k k' : var) (kt : fun_tag) (fv fv1 : list var)
@@ -99,13 +101,14 @@ Inductive uncurry_step : exp -> exp -> Prop :=
   (* (4) misc. let bindings (needed for computation of new ms) *)
   fp_numargs = length fv + length gv /\ ms = ms ->
   (* 'Irrelevant' guard *)
-  When (fun (r : R_misc) (s : S_misc) =>
+  When (fun (is_cps : R_misc) (s : S_misc) =>
+    is_cps &&
     let '(b, aenv, lm, s, cdata) := s in
     (* g must not have been already uncurried by an earlier pass *)
     negb match M.get ![g] lm with
     | Some true => true
     | _ => false
-    end) ->
+    end)%bool ->
   (* The rewrite *)
   uncurry_step
     (C ⟦ Fcons f ft (k :: fv) (Efun (Fcons g gt gv ge Fnil) (Eapp k' kt [g'])) fds ⟧)
@@ -123,9 +126,63 @@ Inductive uncurry_step : exp -> exp -> Prop :=
              (set_names_lst ![fv] ![fv1] ""
              (set_names_lst ![gv] ![gv1] "" cdata))
            in
-           (true, aenv, lm, s, cdata) : S_misc)
+           (b, aenv, lm, s, cdata) : S_misc)
          (* Rewrite f as a wrapper around the uncurried f1 and recur on fds *)
          (Fcons f ft (k :: fv1) (Efun (Fcons g gt gv1 (Eapp f1 ft1 (gv1 ++ fv1)) Fnil) (Eapp k kt [g]))
+         (Fcons f1 ft1 (gv ++ fv) ge (Rec fds))) ⟧)
+(* Uncurrying for ANF *)
+| uncurry_anf :
+  forall (C : frames_t exp_univ_fundefs exp_univ_exp)
+    (f f1 : var) (ft ft1 : fun_tag) (fv fv1 : list var)
+    (g g' : var) (gt : fun_tag) (gv gv1 : list var) (ge : exp) (fds : fundefs)
+    (lhs rhs : fundefs) (s : Ensemble cps.var) (next_x : cps.var)
+    (fp_numargs : nat) (ms : S_misc),
+  (* Non-linear LHS constraints *)
+  g = g' /\
+  (* Guards: *)
+  (* (1) g can't be recursive *)
+  ~ ![g] \in used_vars ![ge] /\
+  (* (2) gv1, fv1, f1 must be fresh and contain no duplicates *)
+  lhs = Fcons f ft fv (Efun (Fcons g gt gv ge Fnil) (Ehalt g')) fds /\
+  rhs = Fcons f ft fv1 (Efun (Fcons g gt gv1 (Eapp f1 ft1 (gv1 ++ fv1)) Fnil) (Ehalt g))
+        (Fcons f1 ft1 (gv ++ fv) ge (Rec fds)) /\
+  s = used_vars (exp_of_proto (C ⟦ lhs ⟧)) /\
+  fresh_copies s gv1 /\ length gv1 = length gv /\
+  fresh_copies (s :|: FromList ![gv1]) fv1 /\ length fv1 = length fv /\
+  ~ ![f1] \in (s :|: FromList ![gv1] :|: FromList ![fv1]) /\
+  (* (3) next_x must be a fresh variable *)
+  fresher_than next_x (s :|: FromList ![gv1] :|: FromList ![fv1] :|: [set ![f1]]) /\
+  (* (4) misc. let bindings (needed for computation of new ms) *)
+  fp_numargs = length fv + length gv /\ ms = ms ->
+  (* 'Irrelevant' guard *)
+  When (fun (is_cps : R_misc) (s : S_misc) =>
+    negb is_cps &&
+    let '(b, aenv, lm, s, cdata) := s in
+    (* g must not have been already uncurried by an earlier pass *)
+    negb match M.get ![g] lm with
+    | Some true => true
+    | _ => false
+    end)%bool ->
+  (* The rewrite *)
+  uncurry_step
+    (C ⟦ Fcons f ft fv (Efun (Fcons g gt gv ge Fnil) (Ehalt g')) fds ⟧)
+    (C ⟦ Put (
+           let '(b, aenv, lm, s, cdata) := ms in
+           (* Set flag to indicate that a rewrite was performed (used to iterate to fixed point) *)
+           let b := true in
+           (* Mark g as uncurried *)
+           let lm := M.set ![g] true lm in
+           (* Update inlining heuristic so inliner knows to inline fully saturated calls to f *)
+           let s := (max (fst s) fp_numargs, (M.set ![f] 1 (M.set ![g] 2 (snd s)))) in
+           (* Hack: update cdata to agree with fresh names generated above *)
+           let cdata :=
+             set_name ![f] ![f1] "_uncurried"
+             (set_names_lst ![fv] ![fv1] ""
+             (set_names_lst ![gv] ![gv1] "" cdata))
+           in
+           (b, aenv, lm, s, cdata) : S_misc)
+         (* Rewrite f as a wrapper around the uncurried f1 and recur on fds *)
+         (Fcons f ft fv1 (Efun (Fcons g gt gv1 (Eapp f1 ft1 (gv1 ++ fv1)) Fnil) (Ehalt g))
          (Fcons f1 ft1 (gv ++ fv) ge (Rec fds))) ⟧).
 
 (** * Uncurrying as a recursive function *)
@@ -164,7 +221,7 @@ Proof.
     | |- EditDelay _ -> _ =>
       clear; simpl; intros; lazymatch goal with H : forall _, _ |- _ => eapply H; try reflexivity; eauto end
     end.
-  (* Obligation 1 of 2: explain how to satisfy side conditions for the rewrite *)
+  (* Obligation 1: uncurry_cps side conditions *)
   - intros. rename X into success, H0 into failure.
     (* Check nonlinearities *)
     destruct k as [k], k' as [k'], g as [g], g' as [g'].
@@ -173,7 +230,7 @@ Proof.
     rewrite Pos.eqb_eq in Hkk', Hgg'.
     (* Check whether g has already been uncurried before *)
     destruct ms as [[[[b aenv] lm] heuristic] cdata] eqn:Hms.
-    destruct (negb (match M.get g lm with Some true => true | _ => false end))
+    destruct (mr && negb (match M.get g lm with Some true => true | _ => false end))%bool
       as [|] eqn:Huncurried; [|exact failure].
     (* Check that {g, k} ∩ vars(ge) = ∅ *)
     destruct (occurs_in_exp g ![ge]) eqn:Hocc_g; [exact failure|]. (* TODO: avoid the conversion *)
@@ -198,7 +255,53 @@ Proof.
     + apply fresher_than_not_In; subst f1; exact Hfresh_fv.
     + apply fresher_than_Union; [|subst; simpl; intros y Hy; inversion Hy; lia].
       eapply fresher_than_monotonic; eauto; lia.
-  (* Obligation 2 of 2: explain how to maintain fresh name invariant across edit *)
+  (* Obligation 2: uncurry_anf side conditions *)
+  - intros. rename X0 into success, H0 into failure.
+    (* Check nonlinearities *)
+    destruct g as [g], g' as [g'].
+    destruct (eq_var g g') eqn:Hgg'; [|exact failure].
+    rewrite Pos.eqb_eq in Hgg'.
+    (* Check whether g has already been uncurried before *)
+    destruct ms as [[[[b aenv] lm] heuristic] cdata] eqn:Hms.
+    destruct (negb mr && negb (match M.get g lm with Some true => true | _ => false end))%bool
+      as [|] eqn:Huncurried; [|exact failure].
+    (* Check that {g, k} ∩ vars(ge) = ∅ *)
+    destruct (occurs_in_exp g ![ge]) eqn:Hocc_g; [exact failure|]. (* TODO: avoid the conversion *)
+    apply bool_true_false in Hocc_g.
+    rewrite occurs_in_exp_iff_used_vars in Hocc_g.
+    (* Generate ft1 + new misc state ms *)
+    pose (fp_numargs := length fv + length gv).
+    destruct (get_fun_tag (N.of_nat fp_numargs) ms) as [ft1 ms'] eqn:Hget_ft.
+    specialize success with (ft1 := ft1) (ms := ms') (fp_numargs := fp_numargs).
+    (* Generate f1, fv1, gv1, next_x *)
+    destruct s as [next_x Hnext_x].
+    clearpose Hxgv1 xgv1 (gensyms next_x gv); destruct xgv1 as [next_x0 gv1].
+    clearpose Hxfv1 xfv1 (gensyms next_x0 fv); destruct xfv1 as [next_x1 fv1].
+    clearpose Hf1 f1 next_x1.
+    specialize success with (f1 := mk_var f1) (fv1 := fv1) (gv1 := gv1) (next_x := (next_x1 + 1)%positive).
+    (* Prove that all the above code actually satisfies the side condition *)
+    edestruct (@gensyms_spec var) as [Hgv_copies [Hfresh_gv Hgv_len]]; try exact Hxgv1; [eassumption|].
+    edestruct (@gensyms_spec var) as [Hfv_copies [Hfresh_fv Hfv_len]]; try exact Hxfv1; [eassumption|].
+    eapply success; repeat match goal with |- _ /\ _ => split end;
+      try solve [reflexivity|eassumption|subst;reflexivity].
+    + apply fresher_than_not_In; subst f1; exact Hfresh_fv.
+    + apply fresher_than_Union; [|subst; simpl; intros y Hy; inversion Hy; lia].
+      eapply fresher_than_monotonic; eauto; lia.
+  (* Obligation 3: explain how to maintain fresh name invariant across uncurry_cps *)
+  - clear; unfold Put, Rec; intros.
+    (* Env is easy, because the uncurryer doesn't need it *)
+    split; [exact tt|].
+    (* For state, need create a fresh variable. Thankfully, we have one: next_x *)
+    exists next_x; repeat match goal with H : _ /\ _ |- _ => destruct H end.
+    eapply fresher_than_antimon; [|eassumption].
+    rewrite used_iso, isoABA, used_app.
+    subst s lhs. change (exp_of_proto ?A) with ![A].
+    rewrite used_iso, isoABA, used_app.
+    unfold used; simpl; unbox_newtypes.
+    do 10 normalize_used_vars'; repeat normalize_sets.
+    repeat rewrite strip_vars_app; repeat normalize_sets.
+    intros arbitrary; repeat rewrite In_or_Iff_Union; tauto.
+  (* Obligation 4: explain how to maintain fresh name invariant across uncurry_anf *)
   - clear; unfold Put, Rec; intros.
     (* Env is easy, because the uncurryer doesn't need it *)
     split; [exact tt|].
@@ -217,32 +320,32 @@ Defined.
 (* Check rw_uncurry. *)
 (* Recursive Extraction rw_uncurry. *)
 
-Lemma uncurry_one (ms : S_misc) (e : exp) (s : S <[]> e)
+Lemma uncurry_one (cps : bool) (ms : S_misc) (e : exp) (s : S <[]> e)
   : option (result exp_univ_exp uncurry_step S_misc (@S) <[]> e).
 Proof.
-  pose (res := run_rewriter' rw_uncurry tt ms e tt tt s); destruct res eqn:Hres.
+  pose (res := run_rewriter' rw_uncurry cps ms e tt tt s); destruct res eqn:Hres.
   exact (let '(b, _, _, _, _) := resSMisc in if b then Some res else None).
 Defined.
 
-Fixpoint uncurry_fuel (n : nat) (ms : S_misc) (e : exp) (s : S <[]> e) {struct n}
+Fixpoint uncurry_fuel (cps : bool) (n : nat) (ms : S_misc) (e : exp) (s : S <[]> e) {struct n}
   : result exp_univ_exp uncurry_step S_misc (@S) <[]> e.
 Proof.
   destruct n as [|n].
   - unshelve econstructor; [exact e|auto|auto|apply Relation_Operators.rt_refl].
-  - pose (res := uncurry_one ms e s).
+  - pose (res := uncurry_one cps ms e s).
     refine (match res with Some res' => _ | None => _ end).
     + destruct res'.
       destruct resSMisc as [[[[_ aenv] lm] st] cdata].
-      destruct (uncurry_fuel n (false, aenv, lm, st, cdata) resTree resState)
+      destruct (uncurry_fuel cps n (false, aenv, lm, st, cdata) resTree resState)
         as [resTree' resState' resSMisc' resProof'].
       unshelve econstructor; [exact resTree'|auto|auto|].
       eapply Relation_Operators.rt_trans; eauto.
     + unshelve econstructor; [exact e|auto|auto|apply Relation_Operators.rt_refl].
 Defined.
 
-Definition uncurry_top (n : nat) (cdata : comp_data) (e : exp) : exp * M.t nat * comp_data.
+Definition uncurry_top (cps : bool) (n : nat) (cdata : comp_data) (e : exp) : exp * M.t nat * comp_data.
 Proof.
-  refine (let '{| resTree := e'; resSMisc := ms |} := uncurry_fuel n _ e _ in _).
+  refine (let '{| resTree := e'; resSMisc := ms |} := uncurry_fuel cps n _ e _ in _).
   - exact (false, M.empty _, M.empty _, (0%nat, (M.empty _)), cdata).
   - exists (1 + max_var ![e] 1)%positive.
     change (![ <[]> ⟦ ?e ⟧ ]) with ![e]; unfold fresher_than.
